Prove 'run_path_loops_of_nice_devil_wins'
That is, if the nice devil wins, the runner's path eventually loops.
In order to prove this we demonstrate an equivalence between the
run states inside the escape square and the cartesian product of three
finite sets. Since that means the set of close run states is finite we
can use the pigeonhole principle to complete the proof.

AngelDevil/Main.lean
@@ -1,9 +1,12 @@
 import Mathlib.Data.Fin.Basic
+import Mathlib.Data.Finset.Card
 import Mathlib.Data.List.Basic
 import Mathlib.Tactic.Linarith
 import AngelDevil.Reduced
 import AngelDevil.Focused
 import AngelDevil.Runner
+import AngelDevil.Dupes
+import AngelDevil.Perimeter
 
 set_option linter.style.longLine false
 
@@ -330,11 +333,10 @@ theorem AM2_7 (p : Nat) : (∃ D : Devil, devil_wins D p) →
 -- Note that this result applies to the entire 'RunPath', not just the runner's journey.
 lemma run_path_trapped_of_nice_devil_wins
   (D : Devil) (p : Nat) (hnice : nice D p) (hdwins : devil_wins' D p) :
-  ∃ N, ∀ n, allowed D (make_run D p n).A →
-  ∀ rs ∈ RunPath D p n, close N (0, 0) (loc rs) := by
+  ∃ N, ∀ n, ∀ rs ∈ RunPath D p n, close N (0, 0) (loc rs) := by
   let ⟨N, htraps⟩ := hdwins
   use N
-  intro n hallowed rs rsmem
+  intro n rs rsmem
   -- First handle the case where n = 0
   by_cases nz : n = 0
   · subst nz
@@ -399,3 +401,118 @@ lemma run_path_trapped_of_nice_devil_wins
   rw [← cell_congr_idx A hsteps (Nat.lt_add_one _), ← last, append_last]
   intro h
   exact run_path_not_eaten_of_nice D p n hnice rs rsmem (List.mem_of_getElem h)
+
+-- Let RS be the run states "close" to the origin
+def RS (N : Nat) : Set RunState :=
+  {rs : RunState | close N (0, 0) (loc rs)}
+
+-- Demonstrate an equivalence between the RunStates in the escape square
+-- and the cartesian product of several Finsets whose cardinalities are known.
+def runstate_equiv (N : Nat) :
+  RS N ≃ Finset.range (2 * N + 1) ×ˢ Finset.range (2 * N + 1) ×ˢ uvec_finset where
+  toFun := fun ⟨rs, rsmem⟩ ↦ ⟨⟨Int.toNat (rs.x + N), Int.toNat (rs.y + N), rs.u⟩, by
+    apply Finset.mem_product.mpr; dsimp
+    constructor
+    · apply Finset.mem_range.mpr
+      have hlexN : 0 ≤ rs.x + N := by
+        apply Int.le_add_of_sub_left_le
+        rw [Int.zero_sub]
+        exact close_origin_negxle N (loc rs) rsmem
+      have hxNle : rs.x + N ≤ 2 * N := by
+        rw [two_mul]
+        apply add_le_add_right
+        exact close_origin_xle N (loc rs) rsmem
+      rw [Int.toNat_lt hlexN, Int.natCast_add, Int.natCast_one]
+      exact Int.lt_add_one_of_le hxNle
+    apply Finset.mem_product.mpr; dsimp
+    constructor
+    · apply Finset.mem_range.mpr
+      have hleyN : 0 ≤ rs.y + N := by
+        apply Int.le_add_of_sub_left_le
+        rw [Int.zero_sub]
+        exact close_origin_negyle N (loc rs) rsmem
+      have hyNle : rs.y + N ≤ 2 * N := by
+        rw [two_mul]
+        apply add_le_add_right
+        exact close_origin_yle N (loc rs) rsmem
+      rw [Int.toNat_lt hleyN, Int.natCast_add, Int.natCast_one]
+      exact Int.lt_add_one_of_le hyNle
+    · exact uvec_finset_mem _
+  ⟩
+  invFun := fun ⟨⟨a, b, u⟩, hmem⟩ ↦ ⟨⟨a - N, b - N, u⟩, by
+    rcases Finset.mem_product.mp hmem with ⟨amem, hmem⟩
+    rcases Finset.mem_product.mp hmem with ⟨bmem, umem⟩
+    have alt := Finset.mem_range.mp amem; dsimp at alt
+    have blt := Finset.mem_range.mp bmem; dsimp at blt
+    apply close_origin_of_bounds
+    unfold loc; dsimp
+    constructor
+    · simp
+    constructor
+    · apply Int.sub_left_le_of_le_add (Int.le_of_lt_add_one _)
+      rw [← two_mul]
+      exact Int.ofNat_lt.mpr alt
+    constructor
+    · simp
+    · apply Int.sub_left_le_of_le_add (Int.le_of_lt_add_one _)
+      rw [← two_mul]
+      exact Int.ofNat_lt.mpr blt
+  ⟩
+  left_inv := by
+    intro ⟨rs, rsmem⟩; dsimp; congr
+    · rw [Int.natCast_toNat_eq_self.mpr, Int.add_sub_cancel]
+      apply Int.le_add_of_sub_left_le
+      rw [zero_sub]
+      exact close_origin_negxle N (loc rs) rsmem
+    · rw [Int.natCast_toNat_eq_self.mpr, Int.add_sub_cancel]
+      apply Int.le_add_of_sub_left_le
+      rw [zero_sub]
+      exact close_origin_negyle N (loc rs) rsmem
+  right_inv := by
+    intro ⟨⟨a, b, u⟩, hmem⟩; dsimp; congr
+    · rw [Int.sub_add_cancel]; rfl
+    · rw [Int.sub_add_cancel]; rfl
+
+-- Use the run states equivalence to show that 'RS N' is a Fintype
+instance (N : Nat) : Fintype (RS N) := by
+  let F := (Finset.range (2 * N + 1) ×ˢ Finset.range (2 * N + 1) ×ˢ uvec_finset)
+  exact Fintype.ofEquiv F (runstate_equiv N).symm
+
+-- Use the run states equivalence to prove the cardinality of RS
+-- NOTE: It was very satisfying to prove this, but we don't actually need it!
+-- We only needed to prove that 'RS N' was a Fintype so we can use its cardinality.
+lemma runstate_card (N : Nat) : (RS N).toFinset.card = (2 * N + 1) * (2 * N + 1) * 4 := by
+  rw [Set.toFinset_card]
+  rw [← Finset.card_eq_of_equiv_fintype (runstate_equiv N).symm]
+  rw [Finset.card_product, Finset.card_product]
+  rw [Finset.card_range, uvec_finset_card, mul_assoc]
+
+-- If the nice devil wins, then a long enough RunPath must eventually loop
+lemma run_path_loops_of_nice_devil_wins
+  (D : Devil) (p : Nat) (hnice : nice D p) (hdwins : devil_wins' D p) :
+  ∃ N, ∀ n, N < (RunPath D p n).length → ¬list_nodupes (RunPath D p n) := by
+  -- First get the size of the escape square
+  rcases run_path_trapped_of_nice_devil_wins D p hnice hdwins with ⟨N, hclose⟩
+  -- Use the cardinality of 'RS N' as the lower bound for the length of the RunPath
+  use (RS N).toFinset.card
+  intro n cardlt
+  let L := (RunPath D p n).length
+  -- Define 'F' as the Finset of all 'Fin L'
+  let F := @Finset.univ (Fin L) _
+  change (RS N).toFinset.card < L at cardlt
+  rw [← Eq.trans Finset.card_univ (Fintype.card_fin L)] at cardlt
+  -- Define a function from F to 'RS N'
+  let f : Fin L → RunState := fun i ↦ (RunPath D p n)[i]
+  -- Show that the image of 'f' is in 'RS N'
+  have hmapsto : Set.MapsTo f F (RS N).toFinset := by
+    intro i _; simp
+    exact hclose n (RunPath D p n)[i] (List.get_mem _ _)
+  -- Use the pigeonhole principle to conclude that the RunPath contains a duplicate state
+  rcases Finset.exists_ne_map_eq_of_card_lt_of_maps_to cardlt hmapsto with ⟨i, _, j, _, inej, hij⟩
+  unfold list_nodupes; push_neg
+  by_cases ilt : i.val < j.val
+  · use i.val, j.val, ilt, j.2
+    exact hij
+  rename' ilt => jle; push_neg at jle
+  use j.val, i.val, lt_of_le_of_ne jle (Fin.val_ne_iff.mpr inej).symm, i.2
+  exact hij.symm
